theories/model/Model.thy
@@ -44,7 +44,7 @@ text "First, we nail down some types.  For ease in getting started, we're using 
 
 type_synonym nodeid = nat
 type_synonym genaddr = nat
-type_synonym property = int
+type_synonym property = nat
 
 
 type_synonym addr = "genaddr \<times> property set"
